Linglib.lean
@@ -1335,7 +1335,6 @@ import Linglib.Semantics.Genericity.NominalMappingParameter
 import Linglib.Semantics.Genericity.SortedOntology
 import Linglib.Semantics.Genericity.Subkinds
 import Linglib.Semantics.Homogeneity.Collective
-import Linglib.Semantics.Homogeneity.Conditional
 import Linglib.Semantics.Homogeneity.Decided
 import Linglib.Semantics.Homogeneity.Defs
 import Linglib.Semantics.Homogeneity.Plural
